proof/theories/Semantics.v
@@ -71,6 +71,9 @@ Fixpoint run_rule (rf : regfile) (is : rule_prog) (p : packet) : option verdict 
       run_rule (set_reg rf dst (data_bitops (rf src) mask xor)) rest p
   | ILookup src _ neg elems :: rest =>
       if xorb neg (data_mem (rf src) elems) then run_rule rf rest p else None
+  | ICounter _ _ :: rest => run_rule rf rest p   (* verdict-neutral *)
+  | INotrack :: rest      => run_rule rf rest p
+  | IReject t c :: _ => Some (Reject t c)
   | IImmediate v :: _ => Some v
   end.
 
